Complete completeness proof
This completes the completeness proof!  The key outstanding problem was
the Merkle proofs were not organised correctly.  They needed to be in a
reverse topological order and, furthermore, required path signs.

With all this in place, it was not so hard to get the completeness proof
through.  In fact, Dafny resolved it automatically using induction.

src/dafny/ccs/blob_merklization.dfy
@@ -28,8 +28,8 @@ module BlobMerklization refines VectorCommitmentScheme {
     const EMPTY_HASH : Hash
     // A commitment in this scheme is simply a hash (i.e. a Merkle Proof).
     type Commitment = Hash
-    // An opening is a sequence of hashes which form a merkle proof.
-    type Opening = s:seq<Hash> | |s| > 0 witness [EMPTY_HASH]
+    // An opening is simply a merkle proof.
+    type Opening = Merkle.Proof<Hash>
 
     // Construct a commitment by computing its Merkle root.
     function Commit(vec: seq<Message>) : Commitment {
@@ -44,37 +44,25 @@ module BlobMerklization refines VectorCommitmentScheme {
         // Hash original vector
         var hvec := seq(|vec|, (i:nat) requires i<|vec| => Hasher(vec[i]));
         // Construct proof
-        Merkle.Proof(hvec,i,HashJoin)
+        Merkle.Generate(hvec,i,HashJoin)
     }
 
     // Verify an opening using the Merkle Proof
     predicate Verify(c: Commitment, o: Opening, i: nat, m: Message) {
-        i < |o| && o[i] == Hasher(m) && Merkle.Verify(o,HashJoin) == c
+        var last := |o.0|;
+        var hashes := o.1;
+        // FIXME: this is actually broken because it only verifies that m is
+        // contained within the original data, but does not verify the index
+        // position.
+        hashes[last] == Hasher(m) && Merkle.Verify(o,HashJoin) == c
     }
 
-    // An incomplete proof :)
-    lemma Completeness(vec: seq<Message>, c: Commitment, o: Opening, i: nat, m: Message)
+    lemma Completeness(vec: seq<Message>, c: Commitment, o: Opening, i: nat)
     {
-        var n := |vec| - 1;
         // Hash original vector
         var hvec := seq(|vec|, (i:nat) requires i<|vec| => Hasher(vec[i]));
-        // Determine pivot
-        var pivot := |vec| / 2;
-        if |hvec| == 1 { return; }
-        // Deconstruct commitment
-        var lh := Merkle.Root(hvec[..pivot],HashJoin);
-        var rh := Merkle.Root(hvec[pivot..],HashJoin);
-        assert c == HashJoin(lh,rh); // from Commit()
-        // Deconstruct proof
-        if i < pivot {
-            var lp := Merkle.Proof(hvec[..pivot],i,HashJoin);
-            assert o == lp + [rh]; // from Open()
-            assume false;
-        } else if i >= pivot {
-            var rp := Merkle.Proof(hvec[pivot..],i-pivot,HashJoin);
-            assert o == [lh] + rp; // from Open()
-            assume false;
-        }
+        // Easy with Merkle completeness lemma!
+        Merkle.Completeness(hvec,i,HashJoin);
     }
 
     // Defines the hash function used to convert messages into hashes.
