src/test/merkle_tests.dfy
@@ -23,6 +23,9 @@ module ByteMerkle {
     // In our scheme, messages and hashes are bytes.
     type byte = n:nat | n < 256
 
+    // A proof is over byte words
+    type Proof = Merkle.Proof<byte>
+
     // A very simple (and definitely not cryptographically strong) hash
     // function.
     function Hash(lhs: byte, rhs: byte) : byte {
@@ -36,15 +39,43 @@ module ByteMerkle {
         Merkle.Root(bytes,Hash)
     }
 
-    function Proof(bytes: seq<byte>, i:nat) : seq<byte>
+    function Generate(bytes: seq<byte>, i:nat) : Proof
     requires |bytes| > 0 && i < |bytes| {
-        Merkle.Proof(bytes,i,Hash)
+        Merkle.Generate(bytes,i,Hash)
     }
 
-    function Verify(proof: seq<byte>) : byte
-    requires |proof| > 0 {
+    function Verify(proof: Proof) : byte {
         Merkle.Verify(proof,Hash)
     }
+
+    // ==============================================================
+    // Proofs
+    // ==============================================================
+
+    // Proof that 0 is in [0]
+    const PROOF_0_0 : Proof := ([],[0])
+    // Proof that 0 is in [0,1]
+    const PROOF_0_01 : Proof := ([false],[1,0])
+    // Proof that 1 is in [0,1]
+    const PROOF_1_01 : Proof := ([true],[0,1])
+    // Proof that 0 is in [0,1,2]
+    const PROOF_0_012 : Proof := ([false],[3,0])
+    // Proof that 1 is in [0,1,2]
+    const PROOF_1_012 : Proof := ([true,false],[0,2,1])
+    // Proof that 2 is in [0,1,2]
+    const PROOF_2_012 : Proof := ([true,true],[0,1,2])
+    // Proof that 0 is in [0,1,2,3]
+    const PROOF_0_0123 : Proof := ([false,false],[1,1,0])
+    // Proof that 1 is in [0,1,2,3]
+    const PROOF_1_0123 : Proof := ([false,true],[1,0,1])
+    // Proof that 2 is in [0,1,2,3]
+    const PROOF_2_0123 : Proof := ([true,false],[1,3,2])
+    // Proof that 3 is in [0,1,2,3]
+    const PROOF_3_0123 : Proof := ([true,true],[1,2,3])
+
+    // ==============================================================
+    // Tests
+    // ==============================================================
 
     method {:test} test_root() {
         AssertAndExpect(Root([0]) == 0);
@@ -59,32 +90,46 @@ module ByteMerkle {
     }
 
     method {:test} test_verify() {
-        AssertAndExpect(Verify([0]) == 0);
-        AssertAndExpect(Verify([1,0]) == 1);
-        assert Merkle.Verify([2,1,0],Hash) == Hash(2,Hash(1,0));
-        AssertAndExpect(Verify([2,1,0]) == 3);
-        // Proof that either 1 or 0 is in [7,2,1,0]
-        assert Merkle.Verify([5,1,0],Hash) == Hash(5,Hash(1,0));
-        AssertAndExpect(Verify([5,1,0]) == 4);
+        AssertAndExpect(Verify(PROOF_0_0) == 0);
+        AssertAndExpect(Verify(PROOF_0_01) == 1);
+        AssertAndExpect(Verify(PROOF_1_01) == 1);
+        AssertAndExpect(Verify(PROOF_0_012) == 3);
+        AssertAndExpect(Verify(PROOF_1_012) == 3);
     }
 
+    // Dafny needs a lot of hand holding here :(
     method {:test} test_proof() {
         // n = 1
-        AssertAndExpect(Proof([0],0) == [0]);
+        AssertAndExpect(Generate([0],0) == PROOF_0_0);
         // n = 2
-        AssertAndExpect(Proof([0,1],0) == [0,1]);
-        AssertAndExpect(Proof([0,1],1) == [0,1]);
+        assert Generate([0,1],0).0 == [false];
+        assert Generate([0,1],0).1 == [1,0];
+        AssertAndExpect(Generate([0,1],0) == PROOF_0_01);
+        assert Generate([0,1],1).0 == [true];
+        assert Generate([0,1],1).1 == [0,1];
+        AssertAndExpect(Generate([0,1],1) == PROOF_1_01);
         // n = 3
-        assert Merkle.Proof([0,1,2],0,Hash) == Merkle.Proof([0],0,Hash) + [Merkle.Root([1,2],Hash)];
-        AssertAndExpect(Proof([0,1,2],0) == [0,3]);
-        AssertAndExpect(Proof([0,1,2],1) == [0,1,2]);
-        AssertAndExpect(Proof([0,1,2],2) == [0,1,2]);
+        assert Root([1,2]) == 3;
+        assert Generate([0,1,2],0).1 == [3,0];
+        AssertAndExpect(Generate([0,1,2],0) == PROOF_0_012);
+        assert Generate([0,1,2],1).0 == [true,false];
+        assert Generate([0,1,2],1).1 == [0,2,1];
+        AssertAndExpect(Generate([0,1,2],1) == PROOF_1_012);
+        assert Generate([0,1,2],2).0 == [true,true];
+        assert Generate([0,1,2],2).1 == [0,1,2];
+        AssertAndExpect(Generate([0,1,2],2) == PROOF_2_012);
         // n = 4
-        assert Merkle.Proof([0,1,2,3],0,Hash) == Merkle.Proof([0,1],0,Hash) + [Merkle.Root([2,3],Hash)];
-        AssertAndExpect(Proof([0,1,2,3],0) == [0,1,1]);
-        assert Merkle.Proof([0,1,2,3],1,Hash) == Merkle.Proof([0,1],0,Hash) + [Merkle.Root([2,3],Hash)];
-        AssertAndExpect(Proof([0,1,2,3],1) == [0,1,1]);
-        AssertAndExpect(Proof([0,1,2,3],2) == [1,2,3]);
-        AssertAndExpect(Proof([0,1,2,3],3) == [1,2,3]);
+        expect Generate([0,1,2,3],0).0 == [false,false];
+        expect Generate([0,1,2,3],0).1 == [1,1,0];
+        AssertAndExpect(Generate([0,1,2,3],0) == PROOF_0_0123);
+        expect Generate([0,1,2,3],1).0 == [false,true];
+        expect Generate([0,1,2,3],1).1 == [1,0,1];
+        AssertAndExpect(Generate([0,1,2,3],1) == PROOF_1_0123);
+        expect Generate([0,1,2,3],2).0 == [true,false];
+        expect Generate([0,1,2,3],2).1 == [1,3,2];
+        AssertAndExpect(Generate([0,1,2,3],2) == PROOF_2_0123);
+        expect Generate([0,1,2,3],3).0 == [true,true];
+        expect Generate([0,1,2,3],3).1 == [1,2,3];
+        AssertAndExpect(Generate([0,1,2,3],3) == PROOF_3_0123);
     }
 }
